Add `Similarity` instances

theories/Data/Vector.v
@@ -644,6 +644,21 @@ Proof.
       * intros i. eapply H_p with (i := FS i).
 Qed.
 
+Inductive Similarity_vec_list (A : Type) : forall n : nat, Similarity (Vector.t A n) (list A) :=
+  | Similarity_vec_list_nil
+    : is_similar_to (VNil) (@L.nil A)
+  | Similarity_vec_list_cons n x xs xs'
+    (xs_corres : is_similar_to xs xs')
+    : is_similar_to (VCons n x xs) (@L.cons A x xs').
+
+Lemma Similarity_vec_list_iff {A : Type} {n : nat} (xs : Vector.t A n) (xs' : list A)
+  : is_similar_to (Similarity := Similarity_vec_list A n) xs xs' <-> V.to_list xs = xs'.
+Proof.
+  split.
+  - intros H_sim. induction H_sim; simpl; f_equal; eauto.
+  - intros <-. induction xs as [ | n x xs IH]; simpl; econs; eauto.
+Qed.
+
 End V.
 
 Ltac introVNil :=
